theories/OGS/Subst.v
@@ -3,7 +3,8 @@ Substitution (§ 4.3)
 =====================
 |*)
 From OGS Require Import Prelude.
-From OGS.Utils Require Import Ctx Psh Rel.
+From OGS.Utils Require Import Psh Rel.
+From OGS.Ctx Require Import All.
 
 Open Scope ctx_scope.
 
@@ -11,21 +12,27 @@ Open Scope ctx_scope.
 Substitution Monoid (Def. 4.9)
 ==============================
 
-The specification of an evaluator will be separated in several steps. First we will ask for a family of values,
-i.e. objects that can be substituted for variables. We formalize well-typed well-scoped substitutions in the
-monoidal style of Fiore et al and Allais et al.
+The specification of an evaluator will be separated in several steps. First we will ask
+for a family of values, i.e. objects that can be substituted for variables. We formalize
+well-typed well-scoped substitutions in the monoidal style of Fiore et al and Allais et al.
 |*)
 
-Class subst_monoid {T} (val : Famₛ T) : Type := {
-  v_var {Γ} : Γ =[val]> Γ ; (* Γ ∋ x -> val Γ x *)
-  v_sub {Γ Δ} : Γ =[val]> Δ -> val Γ ⇒ᵢ val Δ ;
+Class subst_monoid `{CC : context T C} (val : Fam₁ T C) := {
+  v_var : c_var ⇒₁ val ;
+  v_sub : val ⇒₁ ⟦ val , val ⟧₁ ;
 }.
-#[global] Notation "u ⊛ᵥ v" := (v_sub u _ v) (at level 30).
+#[global] Arguments v_var {T _ _ val _} [x Γ].
+#[global] Arguments v_sub {T _ _ val _} [x Γ] v {Δ} a.
+#[global] Notation "v ᵥ⊛ a" := (v_sub v a) (at level 30).
 
-Definition e_comp {T val} {_ : @subst_monoid T val} {Γ1 Γ2 Γ3}
-  : Γ2 =[val]> Γ3 -> Γ1 =[val]> Γ2 -> Γ1 =[val]> Γ3
-  := fun u v => s_map (v_sub u) v.
-#[global] Infix "⊛" := e_comp (at level 14).
+Definition a_id `{subst_monoid T C val} {Γ} : Γ =[val]> Γ
+  := fun _ i => v_var i.
+#[global] Arguments a_id _ _ _ _ _ _ _ /.
+Definition a_comp `{subst_monoid T C val} {Γ1 Γ2 Γ3}
+  : Γ1 =[val]> Γ2 -> Γ2 =[val]> Γ3 -> Γ1 =[val]> Γ3
+  := fun u v _ i => u _ i ᵥ⊛ v.
+#[global] Infix "⊛" := a_comp (at level 14).
+#[global] Arguments a_comp _ _ _ _ _ _ _ _ _ _ _ /.
 
 (*|
 The laws for monoids and modules are pretty straitforward. A specificity is that
@@ -33,16 +40,20 @@ assignments are represented by functions from variables to values, as such their
 well-behaved equality is pointwise equality and we require substitution to respect it.
 |*)
 
-Class subst_monoid_laws {T} (val : Famₛ T) {VM : subst_monoid val} : Prop := {
-  v_sub_proper {Γ Δ}
-    :: Proper (ass_eq Γ Δ ==> forall_relation (fun _ => eq ==> eq)) v_sub ;
-  v_sub_var {Γ1 Γ2} (p : Γ1 =[val]> Γ2)
-    : p ⊛ v_var ≡ₐ p ;
-  v_var_sub {Γ1 Γ2} (p : Γ1 =[val]> Γ2)
-    : v_var ⊛ p ≡ₐ p ;
-  v_sub_sub {Γ1 Γ2 Γ3 Γ4} (p : Γ3 =[val]> Γ4) (q : Γ2 =[val]> Γ3) (r : Γ1 =[val]> Γ2)
-   : p ⊛ (q ⊛ r) ≡ₐ (p ⊛ q) ⊛ r ;
+Class subst_monoid_laws `{CC : context T C} (val : Fam₁ T C) {VM : subst_monoid val} := {
+  v_sub_proper :: Proper (∀ₕ Γ, ∀ₕ _, eq ==> ∀ₕ Δ, asgn_eq Γ Δ ==> eq) v_sub ;
+  v_sub_var {Γ1 Γ2 x} (i : Γ1 ∋ x) (p : Γ1 =[val]> Γ2)
+    : v_var i ᵥ⊛ p = p _ i ;
+  v_var_sub {Γ x} (v : val Γ x)
+    : v ᵥ⊛ a_id = v ;
+  v_sub_sub {Γ1 Γ2 Γ3 x} (v : val Γ1 x) (a : Γ1 =[val]> Γ2) (b : Γ2 =[val]> Γ3)
+   : v ᵥ⊛ (a ⊛ b) = (v ᵥ⊛ a) ᵥ⊛ b ;
 } .
+#[global] Arguments subst_monoid_laws {T C CC} val {VM}.
+
+#[global] Instance v_sub_proper_a `{subst_monoid_laws T C val}
+          {Γ1 Γ2 x} {v : val Γ1 x} : Proper (asgn_eq Γ1 Γ2 ==> eq) (v_sub v).
+Proof. now apply v_sub_proper. Qed.
 
 (*|
 Substitution Module (Def. 4.11)
@@ -52,41 +63,53 @@ Next, we ask for a module over the monoid of values, to represent the configurat
 of the machine.
 |*)
 
-Class subst_module {T} (val : Famₛ T) (conf : Fam T) : Type := {
-  c_sub {Γ Δ} : Γ =[val]> Δ -> conf Γ -> conf Δ ;
+Class subst_module `{CC : context T C} (val : Fam₁ T C) (conf : Fam₀ T C) := {
+  c_sub : conf ⇒₀ ⟦ val , conf ⟧₀ ;
 }.
+#[global] Arguments c_sub {T C CC val conf _} [Γ] c {Δ} a.
+#[global] Notation "c ₜ⊛ a" := (c_sub c a) (at level 30).
 
-#[global] Notation "u ⊛ₜ c" := (c_sub u c) (at level 30).
-
-Class subst_module_laws {T} (val : Famₛ T) (conf : Fam T)
-      {VM : subst_monoid val} {CM : subst_module val conf} : Prop := {
-  c_sub_proper {Γ Δ} :: Proper (ass_eq Γ Δ ==> eq ==> eq) c_sub ;
-  c_var_sub {Γ} (c : conf Γ) : v_var ⊛ₜ c = c ;
-  c_sub_sub {Γ1 Γ2 Γ3} (u : Γ2 =[val]> Γ3) (v : Γ1 =[val]> Γ2) {c}
-    : u ⊛ₜ (v ⊛ₜ c) = (u ⊛ v) ⊛ₜ c ;
+Class subst_module_laws `{CC : context T C} (val : Fam₁ T C) (conf : Fam₀ T C)
+      {VM : subst_monoid val} {CM : subst_module val conf} := {
+  c_sub_proper :: Proper (∀ₕ Γ, eq ==> ∀ₕ Δ, asgn_eq Γ Δ ==> eq) c_sub ;
+  c_var_sub {Γ} (c : conf Γ) : c ₜ⊛ a_id = c ;
+  c_sub_sub {Γ1 Γ2 Γ3} (c : conf Γ1) (a : Γ1 =[val]> Γ2) (b : Γ2 =[val]> Γ3)
+    : c ₜ⊛ (a ⊛ b) = (c ₜ⊛ a) ₜ⊛ b ;
 } .
+
+#[global] Instance c_sub_proper_a `{subst_module_laws T C val conf}
+          {Γ1 Γ2 c} : Proper (asgn_eq Γ1 Γ2 ==> eq) (c_sub c).
+Proof. now apply c_sub_proper. Qed.
 
 (*|
 Derived notions: renamings.
 |*)
 
 Section renaming.
-  Context {T : Type} {val : Famₛ T} {conf : Fam T}.
+  Context `{CC : context T C} {val : Fam₁ T C} {conf : Fam₀ T C}.
   Context {VM : subst_monoid val} {VML : subst_monoid_laws val}.
   Context {CM : subst_module val conf} {CML : subst_module_laws val conf}.
 
-  Definition v_ren {Γ Δ} : Γ ⊆ Δ -> val Γ ⇒ᵢ val Δ :=
-    fun u => v_sub (v_var ⊛ᵣ u) .
+  Definition r_emb {Γ Δ} (r : Γ ⊆ Δ) : Γ =[val]> Δ
+    := fun _ i => v_var (r _ i).
+  #[global] Arguments r_emb {_ _} _ _ /.
 
-  Definition e_ren {Γ1 Γ2 Γ3} : Γ2 ⊆ Γ3 -> Γ1 =[val]> Γ2 -> Γ1 =[val]> Γ3
-    := fun u v => (v_var ⊛ᵣ u) ⊛ v.
+  (* equal to respectively `v_sub ⦿₁ hom_precomp₁ v_var` and
+     `c_sub ⦿₀ hom_precomp₀ v_var` but a bit pedantic *)
+  Definition v_ren : val ⇒₁ ⟦ c_var , val ⟧₁
+    := fun _ _ v _ r => v ᵥ⊛ r_emb r.
+  Definition c_ren : conf ⇒₀ ⟦ c_var , conf ⟧₀
+    := fun _ c _ r => c ₜ⊛ r_emb r.
+  #[global] Arguments v_ren [x Γ] v [Δ] r /.
+  #[global] Arguments c_ren [Γ] v [Δ] r /.
 
-  Definition c_ren {Γ1 Γ2} : Γ1 ⊆ Γ2 -> conf Γ1 -> conf Γ2
-    := fun u c => (v_var ⊛ᵣ u) ⊛ₜ c .
+  Definition a_ren_r {Γ1 Γ2 Γ3} : Γ1 =[val]> Γ2 -> Γ2 ⊆ Γ3 -> Γ1 =[val]> Γ3
+    := fun a r => a ⊛ (r_emb r).
+  #[global] Arguments a_ren_r _ _ _ _ _ _ /.
 End renaming.
-#[global] Notation "r ᵣ⊛ᵥ v" := (v_ren r _ v) (at level 14).
-#[global] Infix "ᵣ⊛" := e_ren (at level 14).
-#[global] Infix "ᵣ⊛ₜ" := c_ren (at level 14).
+#[global] Notation "v ᵥ⊛ᵣ r" := (v_ren v r) (at level 14).
+#[global] Notation "c ₜ⊛ᵣ r" := (c_ren c r) (at level 14).
+#[global] Notation "a ⊛ᵣ r" := (a_ren_r a r) (at level 14).
 
 (*|
 Additional assumptions on how variables behave. We basically ask that the identity
@@ -94,19 +117,26 @@ assignment is injective, that being in its image is stable by renaming and that 
 image is decidable.
 |*)
 
-Variant is_var {T} {val : Famₛ T} {VM : subst_monoid val} {Γ x} : val Γ x -> Type :=
-| IsVar (i : Γ ∋ x) : is_var (v_var x i)
+Variant is_var `{VM : subst_monoid T C val} {Γ x} : val Γ x -> Prop :=
+| Vvar (i : Γ ∋ x) : is_var (v_var i)
 .
-Derive NoConfusion for is_var.
 
-Class var_assumptions {T} (val : Famₛ T) {VM : subst_monoid val} : Type := {
-  v_var_inj {Γ x} (i j : Γ ∋ x) : v_var x i = v_var x j -> i = j ;
-  is_var_dec {Γ x} (v : val Γ x) : is_var v + (is_var v -> False) ;
-  is_var_ren {Γ1 Γ2 x} (v : val Γ1 x) (e : Γ1 ⊆ Γ2) : is_var (e ᵣ⊛ᵥ v) -> is_var v ;
+Lemma ren_is_var `{VM : subst_monoid_laws T C val} {Γ1 Γ2 x} (v : val Γ1 x) (r : Γ1 ⊆ Γ2)
+      : is_var v -> is_var (v ᵥ⊛ᵣ r).
+Proof.
+  intro p; dependent elimination p.
+  cbn; rewrite v_sub_var.
+  econstructor.
+Qed.
+
+Class var_assumptions `{CC : context T C} (val : Fam₁ T C) {VM : subst_monoid val} := {
+  v_var_inj {Γ x} : injective (@v_var _ _ _ _ _ Γ x) ;
+  is_var_dec {Γ x} (v : val Γ x) : decidable (is_var v) ;
+  is_var_ren {Γ1 Γ2 x} (v : val Γ1 x) (r : Γ1 ⊆ Γ2) : is_var (v ᵥ⊛ᵣ r) -> is_var v ;
 }.
 
 Section variables.
-  Context {T : Type} (val : Famₛ T).
+  Context `{CC : context T C} (val : Fam₁ T C).
   Context {VM : subst_monoid val} {VML : subst_monoid_laws val}.
   Context {VA : var_assumptions val}.
 
@@ -114,20 +144,16 @@ Section variables.
   Proof.
     refine (match p as i in is_var v
             return forall w (H : w = v) (q : is_var w), i = rew [is_var] H in q
-            with IsVar i => fun w H q => _
+            with Vvar i => fun w H q => _
             end v eq_refl q).
     dependent elimination q.
     pose proof (v_var_inj _ _ H) as H'.
     now dependent elimination H'; dependent elimination H.
   Qed.
 
-  Lemma ren_is_var {Γ1 Γ2 x} (v : val Γ1 x) (e : Γ1 ⊆ Γ2) : is_var v -> is_var (e ᵣ⊛ᵥ v).
-  Proof.
-    intro p; dependent elimination p.
-    pose proof (v_sub_var (v_var ⊛ᵣ e) _ i) as H.
-    unfold v_ren, e_comp, s_map in *.
-    rewrite H; econstructor.
-  Qed.
+  Lemma is_var_simpl {Γ x} {i : Γ ∋ x} (p : is_var (v_var i)) : p = Vvar i.
+  Proof. apply is_var_irr. Qed.
+
 End variables.
 
 (*|
@@ -135,46 +161,43 @@ A couple derived properties on the constructed operations.
 |*)
 
 Section properties.
-  Context {T : Type} (val : Famₛ T).
+  Context {T C} {CC : context T C} (val : Fam₁ T C).
   Context {VM : subst_monoid val} {VML : subst_monoid_laws val}.
 
-  #[global] Instance e_comp_proper {Γ1 Γ2 Γ3} :
-    Proper (ass_eq Γ2 Γ3 ==> ass_eq Γ1 Γ2 ==> ass_eq Γ1 Γ3) e_comp.
-  Proof.
-    intros ? ? H1 ? ? H2 ? i; unfold e_comp, s_map.
-    now rewrite H1, H2.
-  Qed.
+  #[global] Instance a_comp_proper {Γ1 Γ2 Γ3} :
+    Proper (asgn_eq Γ1 Γ2 ==> asgn_eq Γ2 Γ3 ==> asgn_eq Γ1 Γ3) a_comp.
+  Proof. intros ?? H1 ?? H2 ??; cbn; now rewrite H1, H2. Qed.
 
-  #[global] Instance e_ren_proper {Γ1 Γ2 Γ3} :
-    Proper (ass_eq Γ2 Γ3 ==> ass_eq Γ1 Γ2 ==> ass_eq Γ1 Γ3) e_ren.
-  Proof.
-    intros ? ? H1 ? ? H2; unfold e_ren.
-    apply e_comp_proper; eauto; now rewrite H1.
-  Qed.
+  #[global] Instance r_emb_proper {Γ1 Γ2} : Proper (asgn_eq Γ1 Γ2 ==> asgn_eq Γ1 Γ2) r_emb.
+  Proof. intros ?? H ??; cbn; now rewrite H. Qed.
 
-  Lemma e_comp_ren_r {Γ1 Γ2 Γ3 Γ4} (u : Γ3 =[val]> Γ4) (v : Γ2 =[val]> Γ3) (w : Γ1 ⊆ Γ2)
-    : u ⊛ (v ⊛ᵣ w) ≡ₐ (u ⊛ v) ⊛ᵣ w.
-  Proof.
-    reflexivity.
-  Qed.
+  #[global] Instance a_ren_proper {Γ1 Γ2 Γ3} :
+    Proper (asgn_eq Γ1 Γ2 ==> asgn_eq Γ2 Γ3 ==> asgn_eq Γ1 Γ3) a_ren_r.
+  Proof. intros ?? H1 ?? H2 ??; cbn; now rewrite H1, H2. Qed.
 
-  Lemma e_comp_ren_l {Γ1 Γ2 Γ3 Γ4} (u : Γ3 =[val]> Γ4) (v : Γ2 ⊆ Γ3) (w : Γ1 =[val]> Γ2)
-        : (u ⊛ᵣ v) ⊛ w ≡ₐ u ⊛ (v ᵣ⊛ w).
-  Proof.
-    unfold e_ren; now rewrite v_sub_sub, e_comp_ren_r, v_sub_var.
-  Qed.
+  Lemma a_ren_r_simpl {Γ1 Γ2 Γ3} (r : Γ1 ⊆ Γ2) (a : Γ2 =[val]> Γ3) 
+        : r_emb r ⊛ a ≡ₐ r ᵣ⊛ a .
+  Proof. intros ??; cbn; now rewrite v_sub_var. Qed.
 
-  Lemma v_sub_comp {Γ1 Γ2 Γ3} (u : Γ2 =[val]> Γ3) (v : Γ1 =[val]> Γ2) {x} (w : val Γ1 x) :
-    u ⊛ᵥ (v ⊛ᵥ w) = (u ⊛ v) ⊛ᵥ w.
-  Proof.
-    pose (w' := a_append a_empty w : (∅ ▶ x) =[val]> Γ1).
-    change w with (w' _ Ctx.top).
-    do 2 change (?u ⊛ᵥ ?v _ Ctx.top) with ((u ⊛ v) _ Ctx.top).
-    apply v_sub_sub.
-  Qed.
+  Lemma a_ren_id {Γ} : r_emb r_id ≡ₐ a_id (Γ:=Γ) .
+  Proof. reflexivity. Qed.
 
-  Lemma v_sub_id {Γ1 Γ2} (u : Γ1 =[val]> Γ2) {x} (i : Γ1 ∋ x) : u ⊛ᵥ (v_var x i) = u x i .
-  Proof.
-    apply v_sub_var.
-  Qed.
+  Lemma a_comp_ren {Γ1 Γ2 Γ3 Γ4} (a : Γ1 =[val]> Γ2) (b : Γ2 =[val]> Γ3) (r : Γ3 ⊆ Γ4)
+    : (a ⊛ b) ⊛ᵣ r ≡ₐ a ⊛ (b ⊛ᵣ r).
+  Proof. intros ??; cbn; now rewrite <-v_sub_sub. Qed.
+
+  Lemma a_ren_comp {Γ1 Γ2 Γ3 Γ4} (a : Γ1 =[val]> Γ2) (r : Γ2 ⊆ Γ3) (b : Γ3 =[val]> Γ4)
+    : (a ⊛ᵣ r) ⊛ b ≡ₐ a ⊛ (r ᵣ⊛ b).
+  Proof. intros ??; cbn; now rewrite <-v_sub_sub, a_ren_r_simpl. Qed.
+
+  Lemma a_comp_comp {Γ1 Γ2 Γ3 Γ4} (a : Γ1 =[val]> Γ2) (b : Γ2 =[val]> Γ3)
+                    (c : Γ3 =[val]> Γ4)
+    : (a ⊛ b) ⊛ c ≡ₐ a ⊛ (b ⊛ c).
+  Proof. intros ??; cbn; now rewrite v_sub_sub. Qed.
+
+  Lemma a_comp_id {Γ1 Γ2} (a : Γ1 =[val]> Γ2) : a ⊛ a_id ≡ₐ a .
+  Proof. intros ??; cbn; now rewrite v_var_sub. Qed.
+
+  Lemma a_id_comp {Γ1 Γ2} (a : Γ1 =[val]> Γ2) : a_id ⊛ a ≡ₐ a .
+  Proof. intros ??; cbn. now rewrite v_sub_var. Qed.
 End properties.
