theories/OGS/Machine.v
@@ -21,55 +21,56 @@ straightforward.
 .. coq:: none
 |*)
 From OGS Require Import Prelude.
-From OGS.Utils Require Import Ctx Rel.
+From OGS.Utils Require Import Rel.
+From OGS.Ctx Require Import All.
 From OGS.OGS Require Import Subst Obs.
 From OGS.ITree Require Import Event Eq Delay.
 
-Section withFam.
-  Context {bT : baseT}.
-  Context {bV : baseV}.
-  Context {bC : baseC}.
-  Context {sV : subst_monoid bV}.
-  Context {sC : subst_module bV bC}.
-  Context {oS : observation_structure}.
-
 (*|
 Evaluation structures, telling us how to evaluate a configuration,
- and how to stitch one back together from the data sent by Opponent.
+and how to stitch one back together from the data sent by Opponent.
 |*)
-  Class machine : Type := {
-      eval {Γ} : conf Γ -> delay (nf' Γ) ;
-      app {Γ x} (v : val Γ x) (m : obs x) (r : dom m ⇒ᵥ Γ) : conf Γ ;
-    }.
+Class machine {T} (val : Fam₁ T) (conf : Fam T) (obs : obs_struct T) : Type := {
+  eval : conf ⇒₀ (delay ∘ nf obs val) ;
+  app : (val ∥ obs#val) ⇒₀ conf ;
+}.
+#[global] Arguments eval {_ _ _ _ _} [_].
+#[global] Arguments app {_ _ _ _ _} [_].
 
-  Context {M : machine}.
+Definition eval_to_obs `{machine T val conf obs} : conf ⇒₀ (delay ∘ obs∙) :=
+  fun _ t => then_to_obs (eval t) .
 
-  Definition eval_to_obs {Γ} (t : conf Γ) : delay (obs∙ Γ) :=
-    fmap_delay (obs'_of_nf' Γ) (eval t) .
+Definition app' `{machine T val conf obs} {Γ x} v (o : obs x) (a : dom o =[val]> Γ)
+  := app (Cut v (OFill o a)) .   
+
+Definition emb `{machine T val conf obs} `{subst_monoid T val} : nf obs val ⇒₀ conf
+  := app ⦿₀ (f_cut_map v_var f_id₁) .
+#[global] Arguments emb {_ _ _ _ _ _} [_] _ /.
 
 (*|
 The ≺ relation (Def 6.7)
 |*)
-  Variant head_inst_nostep (u : { x : typ & obs x }) : { x : typ & obs x } -> Prop :=
-  | HeadInst {Γ y} (v : val Γ y) (m : obs y) (e : dom m ⇒ᵥ Γ) (p : is_var v -> False) (i : Γ ∋ projT1 u)
-             : eval_to_obs (app v m e) ≊ ret_delay (projT1 u ,' (i , projT2 u)) ->
-               head_inst_nostep u (y ,' m) .
+Variant head_inst_nostep `{machine T val conf obs} `{subst_monoid T val} 
+        (u : sigT obs) : sigT obs -> Prop :=
+| HeadInst {Γ y} (v : val y Γ) (_ : ¬(is_var v)) (m : obs y) (a : dom m =[val]> Γ)
+      (i : projT1 u ∈ Γ) (_ : eval_to_obs _ (app' v m a) ≊ ret_delay (Cut i (projT2 u)))
+    : head_inst_nostep u (y ,' m) .
 
 (*|
 Axiomatization of the machine
 |*)
-   Class machine_laws : Prop := {
+ Class machine_laws `{machine T val conf obs} `{subst_monoid T val} `{subst_module T val conf}: Prop := {
 
 (*|
-[app] respects [ass_eq], to avoid relying on functional extensionality
+[app] respects [asgn_eq], to avoid relying on functional extensionality
 |*)
-       app_proper {Γ x v m} :: Proper (ass_eq (dom m) Γ ==> eq) (@app _ Γ x v m) ;
+   (*app_proper {Γ x v m} :: Proper (asgn_eq (dom m) Γ ==> eq) (@app _ Γ x v m) ;*)
 
 (*|
 [app] commutes with substitution
 |*)
-        app_sub {Γ1 Γ2 x} (e : Γ1 ⇒ᵥ Γ2) (v : val Γ1 x) (m : obs x) (r : dom m ⇒ᵥ Γ1)
-       : e ⊛ₜ app v m r = app (e ⊛ᵥ v) m (e ⊛ r) ;
+   app_sub {Γ1 Γ2 x} (e : Γ1 =[val]> Γ2) (v : val x Γ1) (m : obs x) (r : dom m =[val]> Γ1)
+   : app' v m r ₜ⊛ e = app' (v ᵥ⊛ e) m (r ⊛ e) ;
 
 (*|
 Core hypothesis over the evaluator (Def 4.23):
@@ -77,16 +78,16 @@ Core hypothesis over the evaluator (Def 4.23):
 is equivalent to
 "Evaluating, then substituting, then evaluating once more"
 |*)
-        eval_sub {Γ Δ} (c : conf Γ) (e : Γ ⇒ᵥ Δ)
-       : eval (e ⊛ₜ c)
-         ≋ bind_delay' (eval c) (fun u => eval (app (e _ (nf'_var u)) (nf'_obs u) (e ⊛ nf'_val u))) ;
+   eval_sub {Γ Δ} (c : conf Γ) (e : Γ =[val]> Δ)
+   : eval (c ₜ⊛ e)
+     ≋ bind_delay' (eval c) (fun n => eval (emb n ₜ⊛ e)) ;
 
 (*|
 Evaluating the embedding of a normal form is equivalent to returning the normal form (Def. 4.7)
 |*)
-     eval_nf_ret {Γ} (u : nf' Γ)
-       : eval (app (v_var _ (nf'_var u)) (nf'_obs u) (nf'_val u))
-         ≋ ret_delay u ;
+   eval_nf_ret {Γ} (u : nf obs val Γ)
+   : eval (emb u)
+     ≋ ret_delay u ;
 
 (*|
 The machine has finite redexes (§ 6.2). Necessary for establishing that the composition
